flip order of arguments to circuit.forAll, add a proof for mapFinRange

Clean/Circuit/Theorems.lean
@@ -329,33 +329,33 @@ theorem bind_forAll {f : Circuit F α} {g : α → Circuit F β} :
 -- definition of `forAll` for circuits which collapses uses the same offset in two places
 
 @[reducible, circuit_norm]
-def forAll (circuit : Circuit F α) (prop : Operations.Condition F) (n : ℕ) :=
+def forAll (circuit : Circuit F α) (n : ℕ) (prop : Operations.Condition F) :=
   (circuit.operations n).forAll n prop
 
 lemma forAll_def {circuit : Circuit F α} {n : ℕ} :
-  circuit.forAll prop n ↔ (circuit.operations n).forAll n prop := by rfl
+  circuit.forAll n prop ↔ (circuit.operations n).forAll n prop := by rfl
 
 theorem bind_forAll' {f : Circuit F α} {g : α → Circuit F β} :
-  (f >>= g).forAll prop n ↔
-    f.forAll prop n ∧ ((g (f.output n)).forAll prop (n + f.local_length n)) := by
+  (f >>= g).forAll n prop ↔
+    f.forAll n prop ∧ ((g (f.output n)).forAll (n + f.local_length n) prop) := by
   have h_ops : (f >>= g).operations n = f.operations n ++ (g (f.output n)).operations (f.final_offset n) := rfl
   simp only [forAll]
   rw [bind_forAll]
 
 theorem constraints_hold.soundness_iff_forAll' {env : Environment F} {circuit : Circuit F α} {n : ℕ} :
-  constraints_hold.soundness env (circuit.operations n) ↔ circuit.forAll {
+  constraints_hold.soundness env (circuit.operations n) ↔ circuit.forAll n {
     assert _ e := env e = 0,
     lookup _ l := l.table.contains (l.entry.map env),
     subcircuit _ _ s := s.soundness env
-  } n := by
+  } := by
   rw [forAll_def, constraints_hold.soundness_iff_forAll n]
 
 theorem constraints_hold.completeness_iff_forAll' {env : Environment F} {circuit : Circuit F α} {n : ℕ} :
-  constraints_hold.completeness env (circuit.operations n) ↔ circuit.forAll {
+  constraints_hold.completeness env (circuit.operations n) ↔ circuit.forAll n {
     assert _ e := env e = 0,
     lookup _ l := l.table.contains (l.entry.map env),
     subcircuit _ _ s := s.completeness env
-  } n := by
+  } := by
   rw [forAll_def, constraints_hold.completeness_iff_forAll n]
 
 -- specializations
